src/syntax/FStar.Syntax.Syntax.fst
@@ -37,6 +37,21 @@ module Err  = FStar.Errors
 module GS   = FStar.GenSym
 module FlatSet  = FStar.Compiler.FlatSet
 
+let pragma_to_string (p:pragma) : string =
+  match p with
+  | ResetOptions None     -> "#reset-options"
+  | ResetOptions (Some s) -> format1 "#reset-options \"%s\"" s
+  | SetOptions s          -> format1 "#set-options \"%s\"" s
+  | PushOptions None      -> "#push-options"
+  | PushOptions (Some s)  -> format1 "#push-options \"%s\"" s
+  | RestartSolver         -> "#restart-solver"
+  | PrintEffectsGraph     -> "#print-effects-graph"
+  | PopOptions            -> "#pop-options"
+
+instance showable_pragma = {
+  show = pragma_to_string;
+}
+
 let rec emb_typ_to_string = function
     | ET_abstract -> "abstract"
     | ET_app (h, []) -> h
@@ -85,6 +100,60 @@ let is_internal_qualifier (q:qualifier) : bool =
       true
   | _ ->
       false
+
+instance showable_indexed_effect_binder_kind : showable indexed_effect_binder_kind = {
+  show = (function
+          | Type_binder -> "Type_binder"
+          | Substitutive_binder -> "Substitutive_binder"
+          | BindCont_no_abstraction_binder -> "BindCont_no_abstraction_binder"
+          | Range_binder -> "Range_binder"
+          | Repr_binder -> "Repr_binder"
+          | Ad_hoc_binder -> "Ad_hoc_binder"
+  );
+}
+
+instance tagged_indexed_effect_binder_kind : tagged indexed_effect_binder_kind = {
+  tag_of = (function
+            | Type_binder -> "Type_binder"
+            | Substitutive_binder -> "Substitutive_binder"
+            | BindCont_no_abstraction_binder -> "BindCont_no_abstraction_binder"
+            | Range_binder -> "Range_binder"
+            | Repr_binder -> "Repr_binder"
+            | Ad_hoc_binder -> "Ad_hoc_binder"
+  );
+}
+
+instance showable_indexed_effect_combinator_kind : showable indexed_effect_combinator_kind = {
+  show = (function
+          | Substitutive_combinator ks -> "Substitutive_combinator " ^ show ks
+          | Substitutive_invariant_combinator -> "Substitutive_invariant_combinator"
+          | Ad_hoc_combinator -> "Ad_hoc_combinator"
+  );
+}
+
+instance tagged_indexed_effect_combinator_kind : tagged indexed_effect_combinator_kind = {
+  tag_of = (function
+            | Substitutive_combinator _ -> "Substitutive_combinator"
+            | Substitutive_invariant_combinator -> "Substitutive_invariant_combinator"
+            | Ad_hoc_combinator -> "Ad_hoc_combinator"
+  );
+}
+
+instance showable_eff_extraction_mode : showable eff_extraction_mode = {
+  show = (function
+          | Extract_none s -> "Extract_none " ^ s
+          | Extract_reify -> "Extract_reify"	
+          | Extract_primitive -> "Extract_primitive"
+  );
+}
+
+instance tagged_eff_extraction_mode : tagged eff_extraction_mode = {
+  tag_of = (function
+            | Extract_none _ -> "Extract_none"
+            | Extract_reify -> "Extract_reify"
+            | Extract_primitive -> "Extract_primitive"
+  );
+}
 
 let mod_name (m: modul) = m.name
 
