src/syntax/print/FStar.Syntax.Print.fsti
@@ -16,9 +16,6 @@ See the License for the specific language governing permissions and
 module FStar.Syntax.Print
 
 open FStar.Compiler.Effect
-open FStar.Compiler.Util
-open FStar.Const
-open FStar.Ident
 open FStar.Syntax.Syntax
 open FStar.Class.Show
 open FStar.Class.PP
@@ -26,48 +23,18 @@ open FStar.Class.PP
 module DsEnv = FStar.Syntax.DsEnv
 module Json = FStar.Json
 
-val term_to_string'       : DsEnv.env -> term -> string
-val comp_to_string'       : DsEnv.env -> comp -> string
-
-val sigelt_to_string'     : DsEnv.env -> sigelt -> string
-val sigelt_to_string_short: sigelt -> string
-
-val binder_to_json        : DsEnv.env -> binder -> Json.json
-val binders_to_json       : DsEnv.env -> binders -> Json.json
-
-val ctx_uvar_to_string_no_reason    : ctx_uvar -> string
-
-val term_to_doc'          : DsEnv.env -> term -> Pprint.document
-val comp_to_doc'          : DsEnv.env -> comp -> Pprint.document
-val sigelt_to_doc'        : DsEnv.env -> sigelt -> Pprint.document
-
-val term_to_doc           : term -> Pprint.document
-val comp_to_doc           : comp -> Pprint.document
-val sigelt_to_doc         : sigelt -> Pprint.document
-
-(* Prints as <u1,..,un>ty instead of a pair *)
-val tscheme_to_string : tscheme -> string
-
-(* document *)
-val eff_decl_to_string    : bool -> eff_decl -> string
-
-(* Prints sugar, 'Implicit _' prints as '#', etc *)
-val bqual_to_string       : bqual -> string
-
-val args_to_string : args -> string
+(* Use the instances if possible! *)
 
 instance val showable_term      : showable term
 instance val showable_univ      : showable universe
 instance val showable_comp      : showable comp
 instance val showable_sigelt    : showable sigelt
-instance val showable_args      : showable args
 instance val showable_bv        : showable bv
 instance val showable_fv        : showable fv
 instance val showable_binder    : showable binder
 instance val showable_uvar      : showable uvar
 instance val showable_ctxu      : showable ctx_uvar
 instance val showable_binding   : showable binding
-instance val showable_pragma    : showable pragma
 instance val showable_subst_elt : showable subst_elt
 instance val showable_branch    : showable branch
 instance val showable_aqual     : showable aqual
@@ -78,10 +45,10 @@ instance val showable_letbinding : showable letbinding
 instance val showable_modul      : showable modul
 instance val showable_ctx_uvar_meta : showable ctx_uvar_meta_t
 instance val showable_metadata  : showable metadata
+instance val showable_decreases_order : showable decreases_order
 instance val showable_cflag     : showable cflag
-instance val showable_indexed_effect_combinator_kind : showable indexed_effect_combinator_kind
-instance val showable_eff_extraction_mode : showable eff_extraction_mode
-instance val showable_sub_eff  : showable sub_eff
+instance val showable_sub_eff   : showable sub_eff
+instance val showable_eff_decl  : showable eff_decl
 
 instance val pretty_term        : pretty term
 instance val pretty_univ        : pretty universe
@@ -92,3 +59,32 @@ instance val pretty_ctxu        : pretty ctx_uvar
 instance val pretty_binder      : pretty binder
 instance val pretty_bv          : pretty bv
 instance val pretty_binding     : pretty binding
+
+(* A "short" version of printing a sigelt. Meant to (usually) be a small string
+suitable to embed in an error message. No need to be fully faithful to
+printing universes, etc, it should just make it clear enough to which
+sigelt it refers to. *)
+val sigelt_to_string_short: sigelt -> string
+
+(* These versions take in a DsEnv to abbreviate names. *)
+val term_to_string'       : DsEnv.env -> term -> string
+val comp_to_string'       : DsEnv.env -> comp -> string
+val sigelt_to_string'     : DsEnv.env -> sigelt -> string
+val term_to_doc'          : DsEnv.env -> term -> Pprint.document
+val comp_to_doc'          : DsEnv.env -> comp -> Pprint.document
+val sigelt_to_doc'        : DsEnv.env -> sigelt -> Pprint.document
+
+(* Prints as <u1,..,un>ty instead of a pair. *)
+val tscheme_to_string : tscheme -> string
+
+(* Prints sugar, 'Implicit _' prints as '#', etc *)
+val bqual_to_string       : bqual -> string
+
+(* Prints arguments as they show up in the source, useful
+for error messages. *)
+val args_to_string : args -> string
+
+(* This should really go elsewhere. *)
+val binders_to_json       : DsEnv.env -> binders -> Json.json
+
+val binder_to_string_with_type : binder -> string
